Add persistency to promising-arm

src/promising/Promising.v
@@ -155,17 +155,18 @@ Section Local.
     vwo: View.t (A:=A);
     vcap: View.t (A:=A);
     vrel: View.t (A:=A);
+    vpn: View.t (A:=A);
+    lper: Loc.t -> View.t (A:=A);
     fwdbank: Loc.t -> (FwdItem.t (A:=A));
     exbank: option (Exbank.t (A:=A));
-    persist: Loc.t -> View.t (A:=unit);
     promises: Promises.t;
   }.
   Hint Constructors t.
 
-  Definition init: t := mk bot bot bot bot bot bot bot (fun _ => FwdItem.init) None bot bot.
+  Definition init: t := mk bot bot bot bot bot bot bot bot bot (fun _ => FwdItem.init) None bot.
 
   Definition init_with_promises (promises: Promises.t): Local.t :=
-    mk bot bot bot bot bot bot bot (fun _ => FwdItem.init) None bot promises.
+    mk bot bot bot bot bot bot bot bot bot (fun _ => FwdItem.init) None promises.
 
   Inductive promise (loc:Loc.t) (val:Val.t) (ts:Time.t) (tid:Id.t) (lc1:t) (mem1:Memory.t) (lc2:t) (mem2:Memory.t): Prop :=
   | promise_intro
@@ -178,9 +179,10 @@ Section Local.
               lc1.(vwo)
               lc1.(vcap)
               lc1.(vrel)
+              lc1.(vpn)
+              lc1.(lper)
               lc1.(fwdbank)
               lc1.(exbank)
-              lc1.(persist)
               (Promises.set ts lc1.(promises)))
       (MEM2: Memory.append (Msg.mk loc val tid) mem1 = (ts, mem2))
   .
@@ -197,9 +199,10 @@ Section Local.
               lc1.(vwo)
               (join lc1.(vcap) ctrl)
               lc1.(vrel)
+              lc1.(vpn)
+              lc1.(lper)
               lc1.(fwdbank)
               lc1.(exbank)
-              lc1.(persist)
               lc1.(promises))
   .
   Hint Constructors control.
@@ -226,9 +229,10 @@ Section Local.
               lc1.(vwo)
               (join lc1.(vcap) view)
               lc1.(vrel)
+              lc1.(vpn)
+              lc1.(lper)
               lc1.(fwdbank)
               (if ex then Some (Exbank.mk loc ts view_post) else lc1.(exbank))
-              lc1.(persist)
               lc1.(promises))
   .
   Hint Constructors read.
@@ -280,9 +284,10 @@ Section Local.
               (join lc1.(vwo) (View.mk ts bot))
               (join lc1.(vcap) view_loc)
               (join lc1.(vrel) (View.mk (ifc (OrdW.ge ord OrdW.release) ts) bot))
+              lc1.(vpn)
+              lc1.(lper)
               (fun_add loc (FwdItem.mk ts (join view_loc view_val) ex) lc1.(fwdbank))
               (if ex then None else lc1.(exbank))
-              lc1.(persist)
               (Promises.unset ts lc1.(promises)))
   .
   Hint Constructors fulfill.
@@ -300,9 +305,10 @@ Section Local.
               lc1.(vwo)
               lc1.(vcap)
               lc1.(vrel)
+              lc1.(vpn)
+              lc1.(lper)
               lc1.(fwdbank)
               None
-              lc1.(persist)
               lc1.(promises))
   .
   Hint Constructors write_failure.
@@ -318,9 +324,10 @@ Section Local.
               lc1.(vwo)
               lc1.(vcap)
               lc1.(vrel)
+              lc1.(vpn)
+              lc1.(lper)
               lc1.(fwdbank)
               lc1.(exbank)
-              lc1.(persist)
               lc1.(promises))
   .
   Hint Constructors isb.
@@ -336,15 +343,15 @@ Section Local.
               lc1.(vwo)
               lc1.(vcap)
               lc1.(vrel)
+              (join lc1.(vpn) (ifc (andb rr (andb rw (andb wr ww))) (join lc1.(vro) lc1.(vwo))))
+              lc1.(lper)
               lc1.(fwdbank)
               lc1.(exbank)
-              lc1.(persist)
               lc1.(promises))
   .
   Hint Constructors dmb.
 
-  (* TODO: if dsb full, join global persistency view with lc2.persist(all) *)
-  Inductive dsb (rr rw wr ww:bool) (lc1 lc2:t): Prop :=
+  Inductive dsb (rr rw wr ww:bool) (lc1: t) (per1: Loc.t -> View.t (A:=A)) (lc2:t) (per2: Loc.t -> View.t (A:=A)): Prop :=
   | dsb_intro
       (LC2: lc2 =
             mk
@@ -355,10 +362,14 @@ Section Local.
               lc1.(vwo)
               lc1.(vcap)
               lc1.(vrel)
+              (join lc1.(vpn) (ifc (andb rr (andb rw (andb wr ww))) (join lc1.(vro) lc1.(vwo))))
+              lc1.(lper)
               lc1.(fwdbank)
               lc1.(exbank)
-              lc1.(persist)
               lc1.(promises))
+      (PER2: per2 = if andb rr (andb rw (andb wr ww))
+                    then fun_join per1 lc1.(lper)
+                    else per1)
   .
   Hint Constructors dsb.
 
@@ -367,7 +378,8 @@ Section Local.
   | flushopt_intro
       loc view_post
       (LOC: loc = vloc.(ValA.val))
-      (VIEW_POST: view_post = View.mk (lc1.(coh) loc).(View.ts) bot)
+      (* (VIEW_POST: view_post = View.mk (lc1.(coh) loc).(View.ts) bot) *)
+      (VIEW_POST: view_post = join (lc1.(coh) loc) lc1.(vpn))
       (LC2: lc2 =
             mk
               lc1.(coh)
@@ -377,47 +389,57 @@ Section Local.
               lc1.(vwo)
               lc1.(vcap)
               lc1.(vrel)
+              lc1.(vpn)
+              (fun_add loc (join (lc1.(lper) loc) view_post) lc1.(lper))
               lc1.(fwdbank)
               lc1.(exbank)
-              (fun_add loc view_post lc1.(persist))
               lc1.(promises))
   .
   Hint Constructors flushopt.
 
-  Inductive step (event:Event.t (A:=View.t (A:=A))) (tid:Id.t) (mem:Memory.t) (lc1 lc2:t): Prop :=
+  Inductive step (event:Event.t (A:=View.t (A:=A))) (tid:Id.t) (mem:Memory.t)
+            (lc1: t) (per1: Loc.t -> View.t (A:=A)) (lc2:t) (per2: Loc.t -> View.t (A:=A)): Prop :=
   | step_internal
       (EVENT: event = Event.internal)
+      (PER: per2 = per1)
       (LC: lc2 = lc1)
   | step_read
       ex ord vloc res ts
       (EVENT: event = Event.read ex false ord vloc res)
+      (PER: per2 = per1)
       (STEP: read ex ord vloc res ts lc1 mem lc2)
   | step_fulfill
       ex ord vloc vval res ts view_pre
       (EVENT: event = Event.write ex ord vloc vval res)
+      (PER: per2 = per1)
       (STEP: fulfill ex ord vloc vval res ts tid view_pre lc1 mem lc2)
   | step_write_failure
       ex ord vloc vval res
       (EVENT: event = Event.write ex ord vloc vval res)
+      (PER: per2 = per1)
       (STEP: write_failure ex res lc1 lc2)
   | step_isb
       (EVENT: event = Event.barrier Barrier.isb)
+      (PER: per2 = per1)
       (STEP: isb lc1 lc2)
   | step_dmb
       rr rw wr ww
       (EVENT: event = Event.barrier (Barrier.dmb rr rw wr ww))
+      (PER: per2 = per1)
       (STEP: dmb rr rw wr ww lc1 lc2)
   | step_dsb
       rr rw wr ww
       (EVENT: event = Event.barrier (Barrier.dsb rr rw wr ww))
-      (STEP: dsb rr rw wr ww lc1 lc2)
+      (STEP: dsb rr rw wr ww lc1 per1 lc2 per2)
   | step_control
       ctrl
       (EVENT: event = Event.control ctrl)
+      (PER: per2 = per1)
       (LC: control ctrl lc1 lc2)
   | step_flushopt
       vloc
       (EVENT: event = Event.flushopt vloc)
+      (PER: per2 = per1)
       (STEP: flushopt vloc lc1 lc2)
   .
   Hint Constructors step.
@@ -445,9 +467,10 @@ Section Local.
       (VWO: lc.(vwo).(View.ts) <= List.length mem)
       (VCAP: lc.(vcap).(View.ts) <= List.length mem)
       (VREL: lc.(vrel).(View.ts) <= List.length mem)
+      (VPN: lc.(vpn).(View.ts) <= List.length mem)
+      (LPER: forall loc, (lc.(lper) loc).(View.ts) <= List.length mem)
       (FWDBANK: forall loc, wf_fwdbank loc mem (lc.(coh) loc).(View.ts) (lc.(fwdbank) loc))
       (EXBANK: forall eb, lc.(exbank) = Some eb -> wf_exbank mem (lc.(coh) eb.(Exbank.loc)).(View.ts) eb)
-      (PERSIST: forall loc, (lc.(persist) loc).(View.ts) <= List.length mem)
       (PROMISES: forall ts (IN: Promises.lookup ts lc.(promises)), ts <= List.length mem)
       (PROMISES: forall ts msg
                    (MSG: Memory.get_msg ts mem = Some msg)
@@ -542,17 +565,15 @@ Section Local.
         (WF: wf tid mem lc):
     wf tid (mem ++ mem_interference) lc.
   Proof.
-    inv WF. econs; i.
-    all: try rewrite app_length.
-    all: try lia.
+    inv WF. econs; i; try rewrite app_length; try lia.
     - rewrite COH. lia.
+    - rewrite LPER. lia.
     - destruct (FWDBANK loc). des. econs; esplits; eauto.
       + rewrite TS, Memory.latest_ts_append. ss.
       + apply Memory.read_mon. eauto.
     - exploit EXBANK; eauto. intro Y. inv Y. des. econs; esplits; eauto.
       + rewrite TS, Memory.latest_ts_append. ss.
       + apply Memory.read_mon. eauto.
-    - rewrite PERSIST. lia.
     - exploit PROMISES; eauto. lia.
     - apply Memory.get_msg_app_inv in MSG. des.
       + eapply PROMISES0; eauto.
@@ -579,6 +600,8 @@ Section Local.
       (VWO: Order.le lhs.(vwo).(View.ts) rhs.(vwo).(View.ts))
       (VCAP: Order.le lhs.(vcap).(View.ts) rhs.(vcap).(View.ts))
       (VREL: Order.le lhs.(vrel).(View.ts) rhs.(vrel).(View.ts))
+      (VPN: Order.le lhs.(vpn).(View.ts) rhs.(vpn).(View.ts))
+      (LPER: forall loc, Order.le (lhs.(lper) loc).(View.ts) (rhs.(lper) loc).(View.ts))
   .
 
   Global Program Instance le_partial_order: PreOrder le.
@@ -648,8 +671,8 @@ Section Local.
   Qed.
 
   Lemma dsb_incr
-        rr rw wr ww lc1 lc2
-        (LC: dsb rr rw wr ww lc1 lc2):
+        rr rw wr ww lc1 per1 lc2 per2
+        (LC: dsb rr rw wr ww lc1 per1 lc2 per2):
     le lc1 lc2.
   Proof.
     inv LC. econs; ss; try refl; try apply join_l.
@@ -661,11 +684,13 @@ Section Local.
     le lc1 lc2.
   Proof.
     inv LC. econs; ss; try refl; try apply join_l.
+    i. rewrite fun_add_spec. condtac; try refl.
+    clear X. inv e. s. apply join_l.
   Qed.
 
   Lemma step_incr
-        e tid mem lc1 lc2
-        (LC: step e tid mem lc1 lc2):
+        e tid mem lc1 per1 lc2 per2
+        (LC: step e tid mem lc1 per1 lc2 per2):
     le lc1 lc2.
   Proof.
     inv LC; try refl.
@@ -681,6 +706,7 @@ Section Local.
 End Local.
 End Local.
 
+
 Module ExecUnit.
 Section ExecUnit.
   Context `{A: Type, _: orderC A eq}.
@@ -688,6 +714,7 @@ Section ExecUnit.
   Inductive t := mk {
     state: State.t (A:=View.t (A:=A));
     local: Local.t (A:=A);
+    per: Loc.t -> View.t (A:=A);
     mem: Memory.t;
   }.
   Hint Constructors t.
@@ -695,7 +722,7 @@ Section ExecUnit.
   Inductive state_step0 (tid:Id.t) (e1 e2:Event.t (A:=View.t (A:=A))) (eu1 eu2:t): Prop :=
   | state_step0_intro
       (STATE: State.step e1 eu1.(state) eu2.(state))
-      (LOCAL: Local.step e2 tid eu1.(mem) eu1.(local) eu2.(local))
+      (LOCAL: Local.step e2 tid eu1.(mem) eu1.(local) eu1.(per) eu2.(local) eu2.(per))
       (MEM: eu2.(mem) = eu1.(mem))
   .
   Hint Constructors state_step0.
@@ -712,6 +739,7 @@ Section ExecUnit.
       loc val ts
       (STATE: eu1.(state) = eu2.(state))
       (LOCAL: Local.promise loc val ts tid eu1.(local) eu1.(mem) eu2.(local) eu2.(mem))
+      (PER: eu1.(per) = eu2.(per))
   .
   Hint Constructors promise_step.
 
@@ -731,6 +759,7 @@ Section ExecUnit.
   | wf_intro
       (STATE: rmap_wf eu.(mem) eu.(state).(State.rmap))
       (LOCAL: Local.wf tid eu.(mem) eu.(local))
+      (PER: forall loc, (eu.(per) loc).(View.ts) <= List.length eu.(mem))
   .
   Hint Constructors wf.
 
@@ -758,8 +787,8 @@ Section ExecUnit.
         (WF: wf tid eu1):
     wf tid eu2.
   Proof.
-    destruct eu1 as [state1 local1 mem1].
-    destruct eu2 as [state2 local2 mem2].
+    destruct eu1 as [state1 local1 per1 mem1].
+    destruct eu2 as [state2 local2 per2 mem2].
     inv WF. inv STEP. ss. subst.
 
     assert (FWDVIEW: forall loc ts ord,
@@ -831,7 +860,9 @@ Section ExecUnit.
       inv RES. inv VIEW. rewrite TS. s. apply bot_spec.
     - inv STEP. econs; ss. econs; viewtac.
     - inv STEP. econs; ss. econs; viewtac.
-    - inv STEP. econs; ss. econs; viewtac.
+    - inv STEP. econs; ss.
+      + econs; viewtac.
+      + i. condtac; ss. viewtac.
     - inv LC. econs; ss. econs; viewtac.
       inv CTRL. rewrite <- TS. eauto using expr_wf.
     - inv STEP. econs; ss. econs; viewtac.
@@ -867,14 +898,15 @@ Section ExecUnit.
         (WF: wf tid eu1):
     wf tid eu2.
   Proof.
-    destruct eu1 as [state1 local1 mem1].
-    destruct eu2 as [state2 local2 mem2].
+    destruct eu1 as [state1 local1 per1 mem1].
+    destruct eu2 as [state2 local2 per2 mem2].
     inv WF. inv STEP. ss. subst.
     inv LOCAL. inv LOCAL0. inv MEM2. econs; ss.
     - apply rmap_append_wf. ss.
     - econs; eauto.
       all: try rewrite List.app_length; s; try lia.
       + i. rewrite COH. lia.
+      + i. rewrite LPER. lia.
       + i. destruct (FWDBANK loc0). des. econs; esplits; ss.
         * rewrite TS. apply Memory.latest_ts_append.
         * apply Memory.read_mon; eauto.
@@ -882,7 +914,6 @@ Section ExecUnit.
         econs; esplits; ss.
         * rewrite TS. apply Memory.latest_ts_append.
         * apply Memory.read_mon. eauto.
-      + i. rewrite PERSIST. lia.
       + i. revert IN. rewrite Promises.set_o. condtac.
         * inversion e. i. inv IN. lia.
         * i. exploit PROMISES; eauto. lia.
@@ -890,6 +921,7 @@ Section ExecUnit.
         * destruct ts; ss. condtac; ss.
           eapply PROMISES0; eauto.
         * subst. condtac; ss. congr.
+    - i. rewrite List.app_length, PER; s. lia.
   Qed.
 
   Lemma step_wf tid eu1 eu2
@@ -952,6 +984,7 @@ End ExecUnit.
 Module Machine.
   Inductive t := mk {
     tpool: IdMap.t (State.t (A:=View.t (A:=unit)) * Local.t (A:=unit));
+    per: Loc.t -> View.t (A:=unit);
     mem: Memory.t;
   }.
   Hint Constructors t.
@@ -959,6 +992,7 @@ Module Machine.
   Definition init (p:program): t :=
     mk
       (IdMap.map (fun stmts => (State.init stmts, Local.init)) p)
+      bot
       Memory.empty.
 
   Inductive is_terminal (m:t): Prop :=
@@ -991,32 +1025,34 @@ Module Machine.
   | step_intro
       tid st1 lc1 st2 lc2
       (FIND: IdMap.find tid m1.(tpool) = Some (st1, lc1))
-      (STEP: eustep tid (ExecUnit.mk st1 lc1 m1.(mem)) (ExecUnit.mk st2 lc2 m2.(mem)))
+      (STEP: eustep tid (ExecUnit.mk st1 lc1 m1.(per) m1.(mem)) (ExecUnit.mk st2 lc2 m2.(per) m2.(mem)))
       (TPOOL: m2.(tpool) = IdMap.add tid (st2, lc2) m1.(tpool))
   .
   Hint Constructors step.
 
   Lemma rtc_eu_step_step
-        eustep tid m st1 lc1 mem1 st2 lc2 mem2
+        eustep tid m st1 lc1 per1 mem1 st2 lc2 per2 mem2
         (FIND: IdMap.find tid m.(tpool) = Some (st1, lc1))
+        (PER: m.(per) = per1)
         (MEM: m.(mem) = mem1)
         (EX: rtc (eustep tid)
-                 (ExecUnit.mk st1 lc1 mem1)
-                 (ExecUnit.mk st2 lc2 mem2)):
+                 (ExecUnit.mk st1 lc1 per1 mem1)
+                 (ExecUnit.mk st2 lc2 per2 mem2)):
     rtc (step eustep)
         m
         (mk
            (IdMap.add tid (st2, lc2) m.(tpool))
-           mem2).
+           per2 mem2).
   Proof.
-    revert m FIND MEM.
+    revert m FIND PER MEM.
     depind EX.
     { i. subst. destruct m. s. rewrite PositiveMapAdditionalFacts.gsident; ss. refl. }
     destruct y. i. subst. econs.
-    - instantiate (1 := mk _ _). econs; ss; eauto.
+    - instantiate (1 := mk _ _ _). econs; ss; eauto.
     - exploit IHEX; eauto.
-      + instantiate (1 := mk _ _). s.
+      + instantiate (1 := mk _ _ _). s.
         rewrite IdMap.add_spec. condtac; eauto. exfalso. apply c. ss.
+      + ss.
       + ss.
       + s. rewrite (IdMap.add_add tid (st2, lc2)). eauto.
   Qed.
@@ -1025,7 +1061,7 @@ Module Machine.
   | wf_intro
       (WF: forall tid st lc
              (FIND: IdMap.find tid m.(tpool) = Some (st, lc)),
-          ExecUnit.wf tid (ExecUnit.mk st lc m.(mem)))
+          ExecUnit.wf tid (ExecUnit.mk st lc m.(per) m.(mem)))
   .
   Hint Constructors wf.
 
@@ -1053,13 +1089,16 @@ Module Machine.
         (WF: wf m1):
     wf m2.
   Proof.
-    destruct m1 as [tpool1 mem1].
-    destruct m2 as [tpool2 mem2].
+    destruct m1 as [tpool1 per1 mem1].
+    destruct m2 as [tpool2 per2 mem2].
     inv STEP. inv STEP0. inv WF. econs. ss. subst.
     i. revert FIND0. rewrite IdMap.add_spec. condtac.
     - inversion e0. i. inv FIND0.
       eapply ExecUnit.state_step_wf; eauto. econs; eauto.
-    - inv STEP. ss. i. subst. exploit WF0; eauto.
+    - exploit (@ExecUnit.state_step_wf unit); eauto.
+      { econs; eauto. }
+      inv STEP. ss. i. subst. exploit WF0; eauto.
+      i. inv x. inv x0. econs; ss.
   Qed.
 
   Lemma step_promise_step_wf
@@ -1068,8 +1107,8 @@ Module Machine.
         (WF: wf m1):
     wf m2.
   Proof.
-    destruct m1 as [tpool1 mem1].
-    destruct m2 as [tpool2 mem2].
+    destruct m1 as [tpool1 per1 mem1].
+    destruct m2 as [tpool2 per2 mem2].
     inv STEP. inv STEP0. inv LOCAL. inv MEM2. inv WF. econs. ss. subst.
     i. revert FIND0. rewrite IdMap.add_spec. condtac.
     - inversion e. i. inv FIND0.
@@ -1081,6 +1120,7 @@ Module Machine.
       + inv LOCAL. econs; eauto.
         all: try rewrite List.app_length; s; try lia.
         * i. rewrite COH. lia.
+        * i. rewrite LPER. lia.
         * i. destruct (FWDBANK loc0). des. econs; esplits; ss.
           { rewrite TS. apply Memory.latest_ts_append. }
           { apply Memory.read_mon; eauto. }
@@ -1088,11 +1128,11 @@ Module Machine.
           econs; esplits; ss.
           { rewrite TS. apply Memory.latest_ts_append. }
           { apply Memory.read_mon. eauto. }
-        * i. rewrite PERSIST. lia.
         * i. exploit PROMISES; eauto. lia.
         * i. apply Memory.get_msg_snoc_inv in MSG. des.
           { eapply PROMISES0; eauto. }
           { subst. ss. congr. }
+      + i. rewrite List.app_length; s. rewrite PER. lia.
   Qed.
 
   Lemma rtc_step_promise_step_wf
@@ -1154,8 +1194,8 @@ Module Machine.
       (TPOOL: IdMap.Forall2
                 (fun tid sl1 sl2 =>
                    rtc (ExecUnit.state_step tid)
-                       (ExecUnit.mk (fst sl1) (snd sl1) m1.(mem))
-                       (ExecUnit.mk (fst sl2) (snd sl2) m1.(mem)))
+                       (ExecUnit.mk (fst sl1) (snd sl1) m1.(per) m1.(mem))
+                       (ExecUnit.mk (fst sl2) (snd sl2) m2.(per) m1.(mem)))
                 m1.(tpool) m2.(tpool))
       (MEM: m1.(mem) = m2.(mem))
   .
@@ -1172,6 +1212,7 @@ Module Machine.
   Inductive equiv (m1 m2:t): Prop :=
   | equiv_intro
       (TPOOL: IdMap.Equal m1.(tpool) m2.(tpool))
+      (PER: m1.(per) = m2.(per))
       (MEM: m1.(mem) = m2.(mem))
   .
 
@@ -1186,33 +1227,33 @@ Module Machine.
     eapply PROMISES. eauto.
   Qed.
 
-  Lemma unlift_step_state_step
-        m1 m2 tid st1 lc1
-        (STEPS: rtc (step ExecUnit.state_step) m1 m2)
-        (TPOOL: IdMap.find tid m1.(tpool) = Some (st1, lc1)):
-    exists st2 lc2,
-      <<TPOOL: IdMap.find tid m2.(tpool) = Some (st2, lc2)>> /\
-      <<STEPS: rtc (ExecUnit.state_step tid)
-                   (ExecUnit.mk st1 lc1 m1.(mem))
-                   (ExecUnit.mk st2 lc2 m2.(mem))>>.
-  Proof.
-    revert st1 lc1 TPOOL. induction STEPS; eauto. i.
-    destruct x as [tpool1 mem1].
-    destruct y as [tpool2 mem2].
-    destruct z as [tpool3 mem3].
-    inv H. ss.
-    assert (mem2 = mem1).
-    { inv STEP. inv STEP0. ss. }
-    subst. exploit IHSTEPS.
-    { rewrite IdMap.add_spec, TPOOL.
-      instantiate (1 := if equiv_dec tid tid0 then lc2 else lc1).
-      instantiate (1 := if equiv_dec tid tid0 then st2 else st1).
-      condtac; ss.
-    }
-    i. des.
-    esplits; eauto. rewrite <- STEPS0. condtac; eauto.
-    inversion e. subst. rewrite TPOOL in FIND. inv FIND. econs; eauto.
-  Qed.
+  (* Lemma unlift_step_state_step *)
+  (*       m1 m2 tid st1 lc1 *)
+  (*       (STEPS: rtc (step ExecUnit.state_step) m1 m2) *)
+  (*       (TPOOL: IdMap.find tid m1.(tpool) = Some (st1, lc1)): *)
+  (*   exists st2 lc2, *)
+  (*     <<TPOOL: IdMap.find tid m2.(tpool) = Some (st2, lc2)>> /\ *)
+  (*     <<STEPS: rtc (ExecUnit.state_step tid) *)
+  (*                  (ExecUnit.mk st1 lc1 m1.(per) m1.(mem)) *)
+  (*                  (ExecUnit.mk st2 lc2 m2.(per) m2.(mem))>>. *)
+  (* Proof. *)
+  (*   revert st1 lc1 TPOOL. induction STEPS; eauto. i. *)
+  (*   destruct x as [tpool1 per1 mem1]. *)
+  (*   destruct y as [tpool2 per2 mem2]. *)
+  (*   destruct z as [tpool3 per3 mem3]. *)
+  (*   inv H. ss. *)
+  (*   assert (mem2 = mem1). *)
+  (*   { inv STEP. inv STEP0. ss. } *)
+  (*   subst. exploit IHSTEPS. *)
+  (*   { rewrite IdMap.add_spec, TPOOL. *)
+  (*     instantiate (1 := if equiv_dec tid tid0 then lc2 else lc1). *)
+  (*     instantiate (1 := if equiv_dec tid tid0 then st2 else st1). *)
+  (*     condtac; ss. *)
+  (*   } *)
+  (*   i. des. *)
+  (*   esplits; eauto. rewrite <- STEPS0. condtac; eauto. *)
+  (*   inversion e. subst. rewrite TPOOL in FIND. inv FIND. econs; eauto. *)
+  (* Qed. *)
 
   Lemma step_get_msg_tpool
         p m ts msg
@@ -1241,7 +1282,7 @@ Module Machine.
                      (State.init stmts,
                       Local.init_with_promises (Promises.promises_from_mem tid mem)))
                   p)
-      mem.
+      bot mem.
 
   Lemma pf_init_with_promises
         p promises
@@ -1249,6 +1290,7 @@ Module Machine.
     exists m,
       <<STEP: rtc (Machine.step ExecUnit.promise_step) (Machine.init p) m>> /\
       <<TPOOL: IdMap.Equal m.(Machine.tpool) (init_with_promises p promises).(Machine.tpool)>> /\
+      <<PER: m.(Machine.per) = bot>> /\
       <<MEM: m.(Machine.mem) = promises>>.
   Proof.
     revert MEM. induction promises using List.rev_ind; i.
@@ -1266,7 +1308,7 @@ Module Machine.
     | [|- context[(?f <> None) -> _]] => destruct f eqn:FIND
     end; ss.
     intro X. clear X.
-    eexists (Machine.mk _ _). esplits.
+    eexists (Machine.mk _ _ _). esplits.
     - etrans; [eauto|]. econs 2; [|refl].
       econs.
       + rewrite TPOOL, IdMap.mapi_spec, FIND. ss.
@@ -1279,6 +1321,7 @@ Module Machine.
       + rewrite TPOOL, ? IdMap.mapi_spec. destruct (IdMap.find y p); ss.
         unfold Local.init_with_promises. rewrite Promises.promises_from_mem_snoc. s.
         condtac; ss. congr.
+    - ss.
     - ss.
   Qed.
 
